Simple_Networks/Simple_Network_Language_Impl.thy
@@ -34,6 +34,75 @@ proof -
   finally show ?thesis .
 qed
 
+lemma map_index'_inj:
+  "L = L'"
+  if "length L = length L'" "map_index' n f L = map_index' n g L'" "set L \<subseteq> S" "set L' \<subseteq> T"
+     "\<forall> i < length L + n. \<forall> x \<in> S. \<forall>y \<in> T. f i x = g i y \<longrightarrow> x = y"
+  using that
+proof (induction "length L" arbitrary: L L' n)
+  case 0
+  then show ?case
+    by simp
+next
+  case (Suc x)
+  from Suc.prems obtain a b L1 L1' where *:
+    "length L1 = x" "length L1' = x" "L = a # L1" "L' = b # L1'"
+    by (smt Suc.hyps(2) length_Suc_conv)
+  show ?case
+    unfolding \<open>L = _\<close> \<open>L' = _\<close>
+    apply (clarsimp, rule conjI)
+    subgoal
+      by (smt *(3,4) Suc.hyps(2) Suc.prems Suc_less_eq add_Suc_shift less_add_Suc2 list.set_intros(1) list_tail_coinc map_index'.simps(2) set_mp)
+    subgoal
+      apply (rule Suc.hyps)
+      using Suc.prems * by auto
+    done
+qed
+
+lemma map_index_inj:
+  "L = L'"
+  if "map_index f L = map_index g L'" "set L \<subseteq> S" "set L' \<subseteq> T"
+     "\<forall> i < length L. \<forall> x \<in> S. \<forall>y \<in> T. f i x = g i y \<longrightarrow> x = y"
+  using that by - (rule map_index'_inj, auto dest: map_index_eq_imp_length_eq)
+
+lemma (in Prod_TA_Defs) trans_broad_alt_def:
+  "trans_broad =
+    {((L, s), g @ concat (map gs ps), Broad a, r @ concat (map rs ps), (L', s'')) |
+    L s L' s' s'' a p l g f r l' gs fs rs ls' ps.
+      a \<in> broadcast  \<and>
+      (l, g, Out a, f, r, l') \<in> trans (N p) \<and>
+      (\<forall>p \<in> set ps. (L ! p, gs p, In a, fs p, rs p, ls' p) \<in> trans (N p)) \<and>
+      (l \<in> commited (N p) \<or> (\<exists>p \<in> set ps. L ! p \<in> commited (N p))
+      \<or> (\<forall>p < n_ps. L ! p \<notin> commited (N p))) \<and>
+      (\<forall>q < n_ps. q \<notin> set ps \<and> p \<noteq> q \<longrightarrow> \<not> (\<exists>g f r l'. (L!q, g, In a, f, r, l') \<in> trans (N q))) \<and>
+      L!p = l \<and>
+      p < length L \<and> set ps \<subseteq> {0..<n_ps} \<and> p \<notin> set ps \<and> distinct ps \<and> sorted ps \<and> ps \<noteq> [] \<and>
+      L' = fold (\<lambda>p L . L[p := ls' p]) ps L[p := l'] \<and> is_upd s f s' \<and> is_upds s' (map fs ps) s'' \<and>
+      L \<in> states \<and> bounded bounds s \<and> bounded bounds s'' \<and>
+      (\<forall>p. p\<notin>set ps \<longrightarrow> gs p = [])
+    }"
+  unfolding trans_broad_def
+proof ((intro Collect_eqI iffI; elims add: more_elims), goal_cases)
+  case prems: (1 x L s L' s' s'' a p l g f r l' gs fs rs ls' ps)
+  let ?gs = "\<lambda>p. if p \<in> set ps then gs p else []"
+  have *[simp]: "concat (map gs ps) = concat (map ?gs ps)"
+    by (simp cong: map_cong)
+  with prems show ?case
+    by (inst_existentials L s L' s' s'' a p l g f r l' ?gs fs rs ls' ps; (assumption | simp))
+next
+  case (2 x L s L' s' s'' a p l g f r l' gs fs rs ls' ps)
+  then show ?case
+    by blast
+qed
+
+(* XXX Move to distribution *)
+text \<open>Stronger version of @{thm Map.map_of_mapk_SomeI}\<close>
+theorem map_of_mapk_SomeI:
+  assumes "inj f"
+    and "map_of t k = Some x"
+  shows "map_of (map (\<lambda>(k, y). (f k, g y)) t) (f k) = Some (g x)"
+  using assms by (induction t) (auto split: if_split_asm dest: injD)
+
 locale Simple_Network_Impl =
   fixes automata ::
     "('s list \<times> ('a act, 's, 'c, int, 'x, int) transition list
@@ -56,12 +125,933 @@ definition
   "B x \<equiv> if x \<in> dom (map_of bounds') then the (map_of bounds' x) else (0, 0)"
 
 definition
-  "automaton_of \<equiv> \<lambda>(commited, trans, inv).
-  (set commited, set trans, default_map_of [] inv)
-  "
+  "automaton_of \<equiv>
+    \<lambda>(commited, trans, inv). (set commited, set trans, default_map_of [] inv)"
 
 sublocale Prod_TA_Defs
   "(set broadcast, map automaton_of automata, map_of bounds')" .
+
+end
+
+paragraph \<open>Mapping through the product construction\<close>
+
+locale Simple_Network_Impl_map =
+  Simple_Network_Impl automata for
+  automata ::
+    "('s list \<times> ('a act, 's, 'c, int, 'x, int) transition list
+      \<times> ('s \<times> ('c, int) cconstraint) list) list" +
+  fixes map_loc :: "nat \<Rightarrow> 's \<Rightarrow> 's1"
+  fixes map_action :: "'a \<Rightarrow> 'a1"
+  fixes map_clock :: "'c \<Rightarrow> 'c1"
+  fixes map_var :: "'x \<Rightarrow> 'x1"
+  fixes map_time :: "int \<Rightarrow> real"
+begin
+
+definition map_ac :: "('c, int) acconstraint \<Rightarrow> ('c1, real) acconstraint" where
+  "map_ac \<equiv> map_acconstraint map_clock map_time"
+
+definition map_cc :: "('c, int) cconstraint \<Rightarrow> ('c1, real) cconstraint" where
+  "map_cc \<equiv> map (map_acconstraint map_clock map_time)"
+
+definition
+  "map_expr \<equiv> map (\<lambda> (x, e). (map_var x, map_exp map_var id e))"
+
+definition map_automaton :: "nat \<Rightarrow> ('s list \<times> ('a act, 's, 'c, int, 'x, int) transition list
+      \<times> ('s \<times> ('c, int) cconstraint) list) \<Rightarrow> _" where
+  "map_automaton i \<equiv> \<lambda>(commited, trans, inv).
+    (map (map_loc i) commited,
+     map (\<lambda>(l, g, a, f, r, l').
+      (map_loc i l, map_cc g, map_act map_action a, map_expr f, map map_clock r, map_loc i l')) trans,
+     map (\<lambda>(s, cc). (map_loc i s, map_cc cc)) inv)"
+
+definition
+  "map_t_single i = (\<lambda>(l, g, a, f, r, l').
+      (map_loc i l, map_cc g, map_act map_action a, map_expr f, map map_clock r, map_loc i l'))"
+
+definition map_single :: "nat \<Rightarrow> ('s set \<times> ('a act, 's, 'c, int, 'x, int) transition set
+      \<times> ('s \<Rightarrow> ('c, int) cconstraint)) \<Rightarrow> _" where
+  "map_single i \<equiv> \<lambda>(commited, trans, inv).
+    (map_loc i ` commited,
+     map_t_single i ` trans,
+     (\<lambda> l. if l \<in> map_loc i ` fst ` set (snd (snd (automata ! i))) then map_cc (inv (the_inv (map_loc i) l)) else []))"
+
+sublocale map: Prod_TA_Defs
+  "(map_action ` set broadcast,
+    map_index (\<lambda> i a. automaton_of (map_automaton i a)) automata,
+    map_of (map (\<lambda>(x, p). (map_var x, p)) bounds'))"
+  .
+
+definition
+  "map_st \<equiv> \<lambda>(L, s).
+    (map_index map_loc L, \<lambda> x. if x \<in> map_var ` dom s then s (the_inv map_var x) else None)"
+
+definition "map_t \<equiv> \<lambda> (l,g,a,r,l').
+  (map_st l,map_cc g,map_label map_action a,map map_clock r,map_st l')"
+
+abbreviation "map_A \<equiv> \<lambda> (T, I). (map_t ` T, map_cc o I o the_inv map_st)"
+
+context
+  assumes map_loc_inj:    "\<forall> i. inj (map_loc i)"
+      and map_var_inj:    "inj map_var"
+      and map_action_inj: "inj map_action"
+      and map_clock_inj:  "inj map_clock"
+      and map_time_inj:   "inj map_time"
+begin
+
+lemma inj_map_st:
+  "inj map_st"
+  unfolding map_st_def
+  apply (rule injI)
+  apply (clarsimp split: prod.split_asm)
+  apply intros
+  subgoal for L1 s1 L2 s2
+    using map_loc_inj by - (rule map_index_inj[where S = UNIV and T = UNIV], auto elim: injD)
+  subgoal for L1 s1 L2 s2
+    apply (rule ext)
+    subgoal for x
+      apply (drule cong[OF _ HOL.refl, where x = "map_var x"])
+      using map_var_inj apply (auto simp add: the_inv_f_f  split: if_split_asm)
+       apply (clarsimp simp: dom_def image_def; metis)+     
+      done
+    done
+  done
+
+lemma N_eq:
+  \<open>N i = automaton_of (automata ! i)\<close> if \<open>i < n_ps\<close>
+  using that unfolding N_def n_ps_def fst_conv snd_conv by (intro nth_map; simp)
+
+lemma covn_N_eq:
+  \<open>N i = automaton_of (automata ! i)\<close> if \<open>i < n_ps\<close>
+  using that unfolding N_def n_ps_def fst_conv snd_conv by (intro nth_map; simp)
+
+lemma L_len[intro, dest]:
+  "length L = n_ps" if "L \<in> states"
+  using that unfolding states_def by simp
+
+context
+begin
+
+private lemma 2:
+  "Simple_Network_Language.conv_A o automaton_of = (\<lambda>(commited, trans, inv).
+    (set commited,
+     set (map Simple_Network_Language.conv_t trans),
+     default_map_of [] (map (\<lambda> (l, g). (l, conv_cc g)) inv)))"
+  apply (rule ext)
+  apply clarsimp
+  unfolding Simple_Network_Language.conv_A_def automaton_of_def
+  apply (clarsimp split: prod.split)
+  unfolding default_map_of_def
+  unfolding FinFun.map_default_def
+  apply (rule ext)
+  subgoal for xs a
+    by (induction xs) auto
+  done
+
+lemma aux_4:
+  "(\<lambda> l. if l \<in> map_loc i ` fst ` set inv then map_cc (default_map_of [] inv (the_inv (map_loc i) l)) else [])
+= default_map_of [] (map (\<lambda> (l, g). (map_loc i l, map_cc g)) inv)"
+  for inv
+  unfolding default_map_of_def FinFun.map_default_def
+  using map_loc_inj
+  apply (intro ext)
+  apply (clarsimp, safe)
+   apply (auto split: option.split simp: the_inv_f_f simp: map_of_eq_None_iff)
+  subgoal for a b v v'
+    by (auto dest: map_of_mapk_SomeI[rotated 1, where f = "map_loc i" and g = map_cc])
+  subgoal
+    by (auto 4 4 dest: map_of_SomeD)
+  done
+
+(*
+lemma aux_4:
+  "map_cc o default_map_of [] inv o the_inv (map_loc i)
+= default_map_of [] (map (\<lambda> (l, g). (map_loc i l, map_cc g)) inv)"
+  for inv
+unfolding default_map_of_def
+  unfolding FinFun.map_default_def
+  apply (rule ext)
+  apply auto
+  apply (auto split: option.split)
+  apply (simp add: map_cc_def)
+  unfolding map_of_eq_None_iff
+
+  sorry
+*)
+
+private lemma 3:
+  "map.n_ps = n_ps"
+  by (simp add: Prod_TA_Defs.n_ps_def)
+
+private lemma 4:
+  "map.N i = map_single i (N i)" if "i < n_ps"
+  using that unfolding n_ps_def Prod_TA_Defs.N_def fst_conv snd_conv
+  apply (subst nth_map_index)
+   apply simp
+  apply (subst nth_map)
+   apply simp
+  unfolding automaton_of_def
+  unfolding map_single_def map_t_single_def
+  unfolding map_automaton_def
+  apply (auto split: prod.split)
+  unfolding comp_def
+  apply (rule aux_4[symmetric])
+  done
+
+private lemma 5:
+  "inv (map.N i) = (\<lambda> l. if l \<in> map_loc i ` fst ` set (snd (snd (automata ! i))) then map_cc (inv (N i) (the_inv (map_loc i) l)) else [])" if "i < n_ps"
+  unfolding 4[OF that] unfolding map_single_def inv_def by (auto split: prod.split)
+
+(*
+private lemma 5:
+  "inv (map.N i) = map_cc o inv (N i) o the_inv (map_loc i)" if "i < n_ps"
+  unfolding 4[OF that] unfolding map_single_def inv_def by (simp split: prod.split)
+*)
+
+private lemma 6:
+  "map.bounds = (\<lambda> x. if x \<in> map_var ` dom bounds then bounds (the_inv map_var x) else None)"
+  unfolding map.bounds_def bounds_def comp_def
+  apply (rule ext)
+  apply (auto simp: map_of_mapk_SomeI[OF map_var_inj] the_inv_f_f[OF map_var_inj])
+  apply (auto simp: map_of_eq_None_iff dom_map_of_conv_image_fst)
+  done
+
+private lemma 7:
+  "trans (map.N i) = map_t_single i ` (trans (N i))"  if "i < n_ps"
+  unfolding 4[OF that] unfolding map_single_def trans_def by (simp split: prod.split)
+
+private lemma 71:
+  "(map_loc i l, map_cc g, map_act map_action a, map_expr u, map map_clock r, map_loc i l')
+  \<in> trans (map.N i)"
+  if "(l, g, a, u, r, l') \<in> trans (N i)" "i < n_ps"
+  using that(1) by (subst 7[OF \<open>i < n_ps\<close>]) (force simp: map_t_single_def)
+
+lemma map_ac_inj:
+  "ac = ac'" if "map_ac ac = map_ac ac'"
+  using map_clock_inj map_time_inj that by (cases ac; cases ac'; auto simp: map_ac_def dest: injD)
+
+lemma map_cc_inj:
+  "cc = cc'" if "map_cc cc = map_cc cc'"
+  using that unfolding map_cc_def map_ac_def[symmetric]
+  by (subst (asm) inj_map_eq_map) (auto simp: map_ac_inj intro: injI)
+
+(*
+private lemma 72:
+  "(map_loc i l, map_cc g, map_act map_action a, map_expr u, map map_clock r, map_loc i l')
+  \<in> trans (map.N i) \<longleftrightarrow> (l, g, a, u, r, l') \<in> trans (N i)
+" if "i < n_ps"
+  using map_loc_inj map_expr_inj 
+  apply (subst 7[OF that])
+  apply (auto simp: map_t_single_def dest: map_cc_inj)
+  subgoal
+    apply (intros add: more_intros)
+     apply assumption
+    apply simp
+    done
+  done
+*)
+
+private lemma 73:
+  "\<exists>l1 g' a' u' r' l1'.
+    l = map_loc i l1 \<and> g = map_cc g' \<and> a = map_act map_action a' \<and>
+    u = map_expr u' \<and> r = map map_clock r' \<and> l' = map_loc i l1' \<and>
+    (l1, g', a', u', r', l1') \<in> trans (N i)"
+  if "(l, g, a, u, r, l')\<in>trans (map.N i)" "i < n_ps"
+  using that(1) by (subst (asm) 7[OF \<open>i < n_ps\<close>]) (force simp: map_t_single_def)
+
+lemma f_the_inv_f:
+  "f (the_inv f x) = x" if "inj f" "x \<in> range f"
+  using that by (auto simp: the_inv_f_f)
+
+lemma 8[simp]:
+  "map.states = map_index map_loc ` states"
+  unfolding map.states_def states_def 3
+  apply safe
+  subgoal for x
+    apply (rule image_eqI[where x = "map_index (\<lambda>i. the_inv (map_loc i)) x"])
+     apply (subst map_index'_comp)
+     apply (rule sym, rule map_index_congL, subst comp_def)
+     apply (intros add: allI impI)
+    subgoal for p
+     apply (rule f_the_inv_f)
+    using map_loc_inj apply blast
+    apply (simp only:)
+    apply (erule allE, erule (1) impE)
+    apply (subst (asm) 7, assumption)
+    apply (force simp: map_t_single_def)
+    done
+  apply (intros add: more_intros)
+  apply simp
+  apply (erule allE, erule (1) impE)
+apply (subst (asm) 7, assumption)
+  unfolding map_t_single_def
+  apply clarsimp
+  apply (erule bexI[rotated])
+  using map_loc_inj
+  apply (auto simp: the_inv_f_f dest: injD)
+  done
+  apply (simp; fail)
+  apply (fastforce dest!: 71)
+  done
+
+private lemma 9:
+  "commited (map.N p) = map_loc p ` commited (N p)" if \<open>p < n_ps\<close>
+  unfolding 4[OF that] unfolding map_single_def commited_def by (simp split: prod.split)
+
+private lemma 10:
+  "map.broadcast = map_action ` set broadcast"
+  unfolding map.broadcast_def by simp
+
+definition
+  "N' p = map.N p"
+
+lemma SilD:
+  assumes "Sil a = map_act map_action a1"
+  obtains a' where "a1 = Sil a'"
+  using assms by (cases a1) auto
+
+lemma map_loc_injD:
+  "x = y" if "map_loc p x = map_loc p y"
+  using that map_loc_inj by (blast dest: injD)
+
+lemma bounded_mapD_aux:
+  assumes "x \<in> dom (\<lambda>x. s (map_var x))"
+  shows "map_var x \<in> dom s"
+  using assms by auto
+
+lemma map_var_bounds':
+  assumes "map_var x \<in> dom map.bounds"
+  shows "x \<in> fst ` set bounds'"
+  using assms unfolding map.bounds_def by (auto dest!: map_of_SomeD injD[OF map_var_inj])
+
+lemma map_of_domD:
+  "\<exists> y. map_of xs x = Some y" if "x \<in> fst ` set xs"
+  apply (fo_rule domD) using that unfolding dom_map_of_conv_image_fst .
+
+lemma map_bounds_bounds':
+  "map.bounds (map_var x) = map_of bounds' x" if "x \<in> fst ` set bounds'"
+  unfolding map.bounds_def using that
+  by (auto simp: Map.map_of_mapk_SomeI[OF map_var_inj] dest!: map_of_domD)
+
+lemma bounded_mapD:
+  "bounded bounds (s \<circ> map_var)" if "bounded map.bounds s"
+  using that unfolding comp_def bounded_def
+  apply elims
+  apply intros
+  subgoal premises prems
+    using prems(1)
+    unfolding map.bounds_def dom_map_of_conv_image_fst bounds_def fst_conv snd_conv
+    by (auto 4 4 dest: injD[OF map_var_inj])
+  subgoal for x
+    apply (drule bounded_mapD_aux)
+    apply simp
+    apply (frule map_var_bounds')
+    apply (drule (1) bspec)
+    apply (auto simp add: bounds_def map_bounds_bounds')
+    done
+  subgoal for x
+    apply (drule bounded_mapD_aux)
+    apply simp
+    apply (frule map_var_bounds')
+    apply (drule (1) bspec)
+    apply (auto simp add: bounds_def map_bounds_bounds')
+    done
+  done
+
+inductive_cases check_bexp_elims:
+  "check_bexp s (bexp.not b) bv"
+  "check_bexp s (bexp.and b1 b2) bv"
+  "check_bexp s (bexp.or b1 b2) bv"
+  "check_bexp s (bexp.imply b1 b2) bv"
+  "check_bexp s (le i x) bv"
+  "check_bexp s (lt i x) bv"
+  "check_bexp s (ge i x) bv"
+  "check_bexp s (eq i x) bv"
+  "check_bexp s (gt i x) bv"
+
+method fprem =
+  (match premises in R: _ \<Rightarrow> \<open>rule R[elim_format]\<close>, assumption)
+
+lemma map_var_check_bexp:
+  "check_bexp (\<lambda>x. s (map_var x)) b bv" if "check_bexp s (map_bexp map_var id b) bv"
+  using that by (induction b arbitrary: bv) (auto intro: check_bexp.intros elim!: check_bexp_elims)
+
+inductive_cases is_val_elims:
+  "is_val s (const c) d"
+  "is_val s (var x)   v"
+  "is_val s (if_then_else b e1 e2) v"
+
+lemma map_var_is_val:
+  "is_val (\<lambda>x. s (map_var x)) e v" if "is_val s (map_exp map_var id e) v"
+  using that
+  by (induction e arbitrary: v) (auto elim!: is_val_elims map_var_check_bexp intro: is_val.intros)
+
+lemma
+  "(m(x\<mapsto>y) o f) = (m o f)(the_inv f x \<mapsto> y)" if "inj f" "x \<in> range f" for f :: "'a \<Rightarrow> 'b"
+  by (rule ext) (auto simp: the_inv_f_f[OF that(1)] f_the_inv_f[OF that])
+
+lemma is_upd_mapD:
+  assumes "is_upd s (map_expr ac) s'"
+  shows "is_upd (s o map_var) ac (s' o map_var)"
+  using assms
+  unfolding is_upd_def map_expr_def comp_def
+  unfolding list_all2_map1
+  apply -
+  apply elims
+  apply (simp split: prod.splits cong: list.rel_cong_simp add: case_prod_conv)
+  subgoal for xs
+    apply (inst_existentials "map (\<lambda> (x, e). (the_inv map_var x, e)) xs")
+    subgoal premises prems
+      using prems(1)
+      apply (induction rule: list_all2_induct)
+       apply simp
+      apply (clarsimp split: prod.split)
+      apply intros
+       apply (simp add: the_inv_f_f[OF map_var_inj])
+      apply (erule map_var_is_val)
+      done
+    subgoal premises prems
+      apply (subgoal_tac "fst ` set xs \<subseteq> range map_var")
+      apply (rule ext)
+      apply (subst fold_map, simp add: comp_def)
+      subgoal for x
+        apply (induction xs arbitrary: s)
+         apply simp
+        apply simp
+        apply (fo_rule cong)
+         apply (fo_rule fold_cong)
+           apply auto
+        apply (rule ext)
+        unfolding fun_upd_def
+        apply (auto simp: the_inv_f_f[OF map_var_inj] injD[OF map_var_inj])
+        done
+      using prems(1)[THEN list_all2_set2]
+      apply auto
+      done
+    done
+  done
+
+lemma bounded_domD:
+  "dom s = dom bounds" if "bounded bounds s"
+  using that unfolding bounded_def ..
+
+lemma dom_map_bounds:
+  "dom map.bounds = map_var ` dom bounds"
+  unfolding map.bounds_def bounds_def by (force simp: dom_map_of_conv_image_fst)
+
+lemma bounded_map_domD:
+  "dom s = map_var ` dom bounds" if "bounded map.bounds s"
+  using that unfolding bounded_def dom_map_bounds ..
+
+lemma
+  "fold (\<lambda>p L . L[p := ls' p]) ps L[p := l'] = fold (\<lambda>p L . L[p := ls' p]) ps (L[p := l'])"
+  if "p \<notin> set ps" for ps ls' p l'
+  using that by (induction ps arbitrary: L) (auto simp: list_update_swap)
+
+lemma map_index_update:
+  "map_index f (xs[i := a]) = map_index f xs[i := f i a]"
+  by (rule nth_equalityI) (auto simp: nth_list_update')
+
+lemma check_bexp_map_var:
+  assumes "check_bexp s b bv"
+  shows
+   "check_bexp (\<lambda>x. if x \<in> map_var ` dom s then s (the_inv map_var x) else None)
+    (map_bexp map_var id b) bv"
+  using assms by induction (auto 4 4 intro: check_bexp.intros simp: the_inv_f_f[OF map_var_inj])
+
+lemma is_val_map_var:
+  assumes "is_val s e v"
+  shows
+    "is_val (\<lambda>x. if x \<in> map_var ` dom s then s (the_inv map_var x) else None)
+    (map_exp map_var id e) v"
+  supply [simp] = the_inv_f_f[OF map_var_inj]
+  using assms
+  apply induction
+  subgoal
+    by (auto intro!: is_val.intros)
+  subgoal
+    by (auto 4 3 intro!: is_val.intros)
+  by (auto intro!: is_val.intros simp: id_def split del: if_split dest!: check_bexp_map_var)
+
+lemma map_bounds_bounds:
+  "the (map.bounds x) = the (bounds (the_inv map_var x))" if "x \<in> map_var ` dom bounds"
+  using that unfolding map.bounds_def bounds_def
+  by (auto simp: the_inv_f_f[OF map_var_inj] map_of_mapk_SomeI[OF map_var_inj])
+
+lemma map_bounds_dom:
+  "the_inv map_var x \<in> dom bounds" if "x \<in> map_var ` dom bounds"
+  using that by (auto simp: the_inv_f_f[OF map_var_inj])
+
+lemma bounded_map_boundsI:
+  assumes "bounded bounds s"
+  shows
+    "bounded map.bounds (\<lambda>x. if x \<in> map_var ` dom s then s (the_inv map_var x) else None)"
+  using assms unfolding bounded_def dom_map_bounds
+  apply (elims; intros)
+  subgoal premises prems
+    using prems(1) by (auto split: if_split_asm) (auto simp: the_inv_f_f[OF map_var_inj])
+  by (auto dest!: map_bounds_dom simp: map_bounds_bounds)
+
+lemma is_upd_mapI:
+  assumes
+    "is_upd s f s'"
+  shows
+    "is_upd (\<lambda>x. if x \<in> map_var ` dom s then s (the_inv map_var x) else None)
+          (map_expr f)
+          (\<lambda>x. if x \<in> map_var ` dom s' then s' (the_inv map_var x) else None)"
+  using assms
+  unfolding is_upd_def
+  apply elims
+  subgoal for xs
+    apply (inst_existentials "map (\<lambda> (x, v). (map_var x, v)) xs")
+    subgoal premises prems
+      using prems(1)
+      by (induction rule: list_all2_induct) (auto intro: is_val_map_var simp: map_expr_def)
+    subgoal premises prems
+      unfolding \<open>s' = _\<close>
+      apply (rule ext)
+      apply auto
+      subgoal for x
+        apply (induction xs arbitrary: s)
+         apply auto
+        apply (fo_rule cong, fo_rule fold_cong, rule ext)
+           apply (auto simp: the_inv_f_f[OF map_var_inj])
+        done
+      subgoal for x
+        apply (induction xs arbitrary: s)
+         apply (simp; fail)
+        subgoal premises prems for a xs s
+          using prems(2)
+          apply simp
+          apply (cases a)
+          apply (subst prems(1)[of "(\<lambda>(x, v). s(x \<mapsto> v)) a"])
+           apply (simp; fail)
+          apply (fo_rule cong, fo_rule fold_cong, rule ext)
+             apply (auto simp: the_inv_f_f[OF map_var_inj])
+          done
+        done
+      done
+    done
+  done
+
+lemma map_trans_int:
+  "map.trans_int = map_t ` trans_int"
+  unfolding map.trans_int_def trans_int_def
+  supply [simp] = L_len
+  apply standard
+  subgoal
+    apply (clarsimp simp: map_t_def map_t_single_def 3 7 9)
+    apply (rule SilD, assumption)
+    apply (drule map_loc_injD[THEN sym])
+    apply simp
+    apply (drule is_upd_mapD)
+    apply (frule bounded_mapD, drule bounded_map_domD)
+    apply (frule bounded_mapD, drule bounded_map_domD)
+    apply (intros add: more_intros)
+            apply solve_triv+
+          apply (auto dest: map_loc_injD; fail)
+         apply solve_triv+
+    subgoal
+      unfolding map_st_def
+      by (auto 4 4 simp: the_inv_f_f[OF map_var_inj] map_index_update[symmetric] intro!: ext)
+    done
+  subgoal
+    apply (rule subsetI, clarsimp simp: Simple_Network_Language.conv_t_def 3 7 9)
+    unfolding map_t_def
+    apply (simp add: map_st_def map_index_update)
+    apply (drule (1) 71)
+    apply (drule is_upd_mapI)
+    apply (drule bounded_map_boundsI)+
+    apply (intros add: more_intros)
+          apply solve_triv+
+        apply (auto dest: map_loc_injD simp: 9; fail)
+       apply solve_triv+
+    done
+  done
+
+lemma InD:
+  assumes "In a = map_act map_action a1"
+  obtains a' where "a1 = In a'"
+  using assms by (cases a1) auto
+
+lemma OutD:
+  assumes "Out a = map_act map_action a1"
+  obtains a' where "a1 = Out a'"
+  using assms by (cases a1) auto
+
+lemma map_cc_append:
+  "map_cc (g1 @ g2) = map_cc g1 @ map_cc g2"
+  unfolding map_cc_def by simp
+
+lemma map_trans_bin:
+  "map.trans_bin = map_t ` trans_bin"
+unfolding map.trans_bin_def trans_bin_def
+  supply [simp] = L_len
+  apply standard
+  subgoal
+    apply (clarsimp simp: map_t_def map_t_single_def 3 7 9)
+    apply (rule InD, assumption)
+    apply (rule OutD, assumption)
+    apply (drule map_loc_injD[THEN sym])
+    apply (drule map_loc_injD[THEN sym])
+    apply (simp add: injD[OF map_action_inj])
+    apply (drule injD[OF map_action_inj])
+    apply (drule is_upd_mapD)
+    apply (drule is_upd_mapD)
+    apply (frule bounded_mapD, drule bounded_map_domD)
+    apply (frule bounded_mapD, drule bounded_map_domD)
+    apply (intros add: more_intros)
+                  apply solve_triv+
+                apply (auto dest: map_loc_injD; fail)
+                apply solve_triv+
+    subgoal
+      unfolding map_st_def
+      by (auto 4 3
+          simp: the_inv_f_f[OF map_var_inj] map_index_update[symmetric] map_cc_def intro!: ext)
+      done
+  subgoal
+    apply (rule subsetI, clarsimp simp: Simple_Network_Language.conv_t_def 3 7 9)
+    unfolding map_t_def
+    apply (simp add: map_st_def map_index_update map_cc_append)
+    apply (drule (1) 71)+
+    apply (drule is_upd_mapI)+
+    apply (drule bounded_map_boundsI)+
+    apply (intros add: more_intros)
+          apply solve_triv+
+        apply (auto dest: map_loc_injD simp: 9; fail)
+       apply solve_triv+
+    done
+  done
+
+lemma n_ps_rangeD:
+  "p < n_ps" if "p \<in> set ps" "set ps \<subseteq> {0..<n_ps}"
+  using that by auto
+
+lemma map_cc_concat:
+  "map_cc (concat gs) = concat (map map_cc gs)"
+  unfolding map_cc_def by (simp add: map_concat)
+
+private lemma 711:
+  "(map_index map_loc L ! i, map_cc g, map_act map_action a, map_expr u, map map_clock r, map_loc i l')
+  \<in> trans (map.N i)"
+  if "(L ! i, g, a, u, r, l') \<in> trans (N i)" "i < n_ps" "length L = n_ps"
+  using 71[OF that(1,2)] that(2,3) by simp
+
+lemma is_upds_mapI:
+  assumes "is_upds s' (map fs ps) s''"
+  shows
+  "is_upds (\<lambda>x. if x \<in> map_var ` dom s' then s' (the_inv map_var x) else None)
+        (map (\<lambda>a. map_expr (fs a)) ps)
+        (\<lambda>x. if x \<in> map_var ` dom s'' then s'' (the_inv map_var x) else None)"
+  sorry
+
+lemma map_trans_broad_aux1:
+  "map_index map_loc (fold (\<lambda>p L. L[p := ls' p]) ps L) =
+  fold (\<lambda>p L. L[p := map_loc p (ls' p)]) ps (map_index map_loc L)"
+  by (induction ps arbitrary: L) (auto simp: map_index_update)
+
+lemma InD2:
+  assumes "In (map_action a) = map_act map_action a'"
+  shows "a' = In a"
+  using assms by (cases a')  (auto simp: injD[OF map_action_inj])
+
+lemma map_trans_broad:
+  "map.trans_broad = map_t ` trans_broad"
+  unfolding map.trans_broad_alt_def trans_broad_alt_def
+  apply standard
+   supply [simp] = L_len
+  subgoal sorry
+  subgoal
+    apply (rule subsetI)
+    apply (clarsimp simp:
+        Simple_Network_Language.conv_t_def 3 7 9 10 map_concat broadcast_def)
+    unfolding map_t_def
+    apply (drule (1) 711, (simp; fail))
+    apply (drule is_upd_mapI is_upds_mapI bounded_map_boundsI)+
+    apply (simp add: map_st_def map_index_update map_cc_append map_cc_concat map_trans_broad_aux1)
+    apply (intros add: more_intros)
+                   apply solve_triv+
+                  apply (simp add: map_concat; fail)
+                 apply solve_triv+
+               apply (drule(1) bspec, drule 711, force, simp, simp)
+    subgoal premises prems for a b aa ab ac ad ba L s s' s'' aj p g f r l' gs fs rs ls' ps
+      using prems(4) \<open>p < n_ps\<close> \<open>set ps \<subseteq> _\<close> \<open>L \<in> states\<close> by (force dest: map_loc_injD simp: 9)
+    subgoal premises prems for a b aa ab ac ad ba L s s' s'' aj p g f r l' gs fs rs ls' ps q
+      using prems(5) \<open>q < n_ps\<close> \<open>q \<notin> set ps \<and> p \<noteq> q\<close> \<open>L \<in> states\<close>
+      by (auto dest!: map_loc_injD InD2 simp: map_t_single_def)
+            apply solve_triv+
+           apply force
+          apply solve_triv+
+    apply (simp add: map_cc_def)
+    done
+
+lemma map_prod_ta:
+  "map.prod_ta = map_A prod_ta"
+  unfolding map.prod_ta_def prod_ta_def
+  unfolding map.trans_prod_def trans_prod_def
+  unfolding map.prod_inv_def prod_inv_def
+  unfolding map.N_def N_def 3
+  apply simp
+  apply (rule conjI)
+  subgoal
+    unfolding image_Un
+    by ((fo_rule arg_cong2)+; rule map_trans_int map_trans_bin map_trans_broad)
+  subgoal \<comment>\<open>Invariant\<close>
+    unfolding map.N_def N_def
+    by (rule ext) (auto simp: 5 map_concat intro!: map_cong arg_cong[where f = concat])
+  done
+
+end (* Injectivity *)
+
+end (* Mapping *)
+
+
+
+paragraph \<open>Conversion from integers to reals commutes with product construction.\<close>
+
+sublocale conv: Prod_TA_Defs
+  "(set broadcast, map (Simple_Network_Language.conv_A o automaton_of) automata, map_of bounds')" .
+
+lemma (in -) conv_ac_inj:
+  "ac = ac'" if "conv_ac ac = conv_ac ac'"
+  using that by (cases ac; cases ac'; auto)
+
+lemma (in -) conv_cc_inj:
+  "cc = cc'" if "conv_cc cc = conv_cc cc'"
+  using that by (subst (asm) inj_map_eq_map) (auto simp add: conv_ac_inj intro: injI)
+
+lemma (in Prod_TA_Defs) trans_broad_alt_def:
+  "trans_broad =
+    {((L, s), g @ concat (map gs ps), Broad a, r @ concat (map rs ps), (L', s'')) |
+    L s L' s' s'' a p l g f r l' gs fs rs ls' ps.
+      a \<in> broadcast  \<and>
+      (l, g, Out a, f, r, l') \<in> trans (N p) \<and>
+      (\<forall>p \<in> set ps. (L ! p, gs p, In a, fs p, rs p, ls' p) \<in> trans (N p)) \<and>
+      (l \<in> commited (N p) \<or> (\<exists>p \<in> set ps. L ! p \<in> commited (N p))
+      \<or> (\<forall>p < n_ps. L ! p \<notin> commited (N p))) \<and>
+      (\<forall>q < n_ps. q \<notin> set ps \<and> p \<noteq> q \<longrightarrow> \<not> (\<exists>g f r l'. (L!q, g, In a, f, r, l') \<in> trans (N q))) \<and>
+      L!p = l \<and>
+      p < length L \<and> set ps \<subseteq> {0..<n_ps} \<and> p \<notin> set ps \<and> distinct ps \<and> sorted ps \<and> ps \<noteq> [] \<and>
+      L' = fold (\<lambda>p L . L[p := ls' p]) ps L[p := l'] \<and> is_upd s f s' \<and> is_upds s' (map fs ps) s'' \<and>
+      L \<in> states \<and> bounded bounds s \<and> bounded bounds s'' \<and>
+      (\<forall>p. p\<notin>set ps \<longrightarrow> gs p = [])
+    }"
+  unfolding trans_broad_def
+proof ((intro Collect_eqI iffI; elims add: more_elims), goal_cases)
+  case prems: (1 x L s L' s' s'' a p l g f r l' gs fs rs ls' ps)
+  let ?gs = "\<lambda>p. if p \<in> set ps then gs p else []"
+  have *[simp]: "concat (map gs ps) = concat (map ?gs ps)"
+    by (simp cong: map_cong)
+  with prems show ?case
+    by (inst_existentials L s L' s' s'' a p l g f r l' ?gs fs rs ls' ps; (assumption | simp))
+next
+  case (2 x L s L' s' s'' a p l g f r l' gs fs rs ls' ps)
+  then show ?case
+    by blast
+qed
+
+lemma N_eq:
+  \<open>N i = automaton_of (automata ! i)\<close> if \<open>i < n_ps\<close>
+  using that unfolding N_def n_ps_def fst_conv snd_conv by (intro nth_map; simp)
+
+lemma covn_N_eq:
+  \<open>N i = automaton_of (automata ! i)\<close> if \<open>i < n_ps\<close>
+  using that unfolding N_def n_ps_def fst_conv snd_conv by (intro nth_map; simp)
+
+lemma L_len[intro, dest]:
+  "length L = n_ps" if "L \<in> states"
+  using that unfolding states_def by simp
+
+context
+begin
+
+private lemma 1:
+  "conv (set broadcast, map automaton_of automata, map_of bounds') =
+    (set broadcast, map (Simple_Network_Language.conv_A o automaton_of) automata, map_of bounds')"
+  unfolding conv_def by simp
+
+private lemma 2:
+  "Simple_Network_Language.conv_A o automaton_of = (\<lambda>(commited, trans, inv).
+    (set commited,
+     set (map Simple_Network_Language.conv_t trans),
+     default_map_of [] (map (\<lambda> (l, g). (l, conv_cc g)) inv)))"
+  apply (rule ext)
+  apply clarsimp
+  unfolding Simple_Network_Language.conv_A_def automaton_of_def
+  apply (clarsimp split: prod.split)
+  unfolding default_map_of_def
+  unfolding FinFun.map_default_def
+  apply (rule ext)
+  subgoal for xs a
+    by (induction xs) auto
+  done
+
+private lemma 3:
+  "conv.n_ps = n_ps"
+  by (simp add: Prod_TA_Defs.n_ps_def)
+
+private lemma 4:
+  "conv.N i = Simple_Network_Language.conv_A (N i)" if "i < n_ps"
+  using that unfolding n_ps_def Prod_TA_Defs.N_def fst_conv snd_conv by (subst nth_map | simp)+
+
+private lemma 5:
+  "inv (conv.N i) = conv_cc o (inv (N i))" if "i < n_ps"
+  unfolding 4[OF that] unfolding Simple_Network_Language.conv_A_def by (simp split: prod.split)
+
+private lemma 6[simp]:
+  "conv.bounds = bounds"
+  unfolding conv.bounds_def bounds_def by simp
+
+private lemma 7:
+  "trans (conv.N i) = Simple_Network_Language.conv_t ` (trans (N i))"  if "i < n_ps"
+  unfolding 4[OF that] unfolding Simple_Network_Language.conv_A_def by (simp split: prod.split)
+
+private lemma 71:
+  "(l, conv_cc g, a, r, u, l')\<in>Simple_Network_Language.trans (conv.N i)"
+  if "(l, g, a, r, u, l')\<in>Simple_Network_Language.trans (N i)" "i < n_ps"
+  using that by (force simp add: 7 Simple_Network_Language.conv_t_def)
+
+private lemma 72:
+  "(l, conv_cc g, a, r, u, l')\<in>Simple_Network_Language.trans (conv.N i)
+\<longleftrightarrow> (l, g, a, r, u, l')\<in>Simple_Network_Language.trans (N i)
+" if "i < n_ps"
+  apply (auto simp add: 7[OF that] Simple_Network_Language.conv_t_def dest: conv_cc_inj)
+  subgoal
+    apply (intros add: more_intros)
+     apply assumption
+    apply simp
+    done
+  done
+
+private lemma 73:
+  "\<exists>g'. g = conv_cc g' \<and> (l, g', a, r, u, l')\<in>Simple_Network_Language.trans (N i)"
+  if "(l, g, a, r, u, l')\<in>Simple_Network_Language.trans (conv.N i)" "i < n_ps"
+  using that by (force simp add: 7 Simple_Network_Language.conv_t_def)
+
+lemma 8[simp]:
+  "conv.states = states"
+  unfolding conv.states_def states_def 3
+  by (auto simp add: 7 Simple_Network_Language.conv_t_def) (fastforce, force)
+
+private lemma 9:
+  "commited (conv.N p) = commited (N p)" if \<open>p < n_ps\<close>
+  unfolding 4[OF that] unfolding Simple_Network_Language.conv_A_def by (simp split: prod.split)
+
+private lemma 10:
+  "conv.broadcast = set broadcast"
+  unfolding conv.broadcast_def by simp
+
+lemma conv_trans_int:
+  "conv.trans_int = (\<lambda>(l, g, a, r, l'). (l, map conv_ac g, a, r, l')) ` trans_int"
+  unfolding conv.trans_int_def trans_int_def
+  supply [simp] = L_len
+  apply standard
+  subgoal
+    by (clarsimp simp: Simple_Network_Language.conv_t_def 3 7 9)
+      (intros add: more_intros, solve_triv+)
+  subgoal
+    by (rule subsetI, clarsimp simp: Simple_Network_Language.conv_t_def 3 7 9[symmetric])
+      ((drule (1) 71)+, intros add: more_intros, solve_triv+)
+  done
+
+lemma conv_trans_bin:
+  "conv.trans_bin = (\<lambda>(l, g, a, r, l'). (l, map conv_ac g, a, r, l')) ` trans_bin"
+  unfolding conv.trans_bin_def trans_bin_def
+  supply [simp] = L_len
+  apply standard
+  subgoal
+    by (clarsimp simp add: Simple_Network_Language.conv_t_def 3 7 9)
+      (intros add: more_intros, solve_triv+)
+  subgoal
+    by (rule subsetI, clarsimp simp add: Simple_Network_Language.conv_t_def 3 7 9[symmetric])
+      ((drule (1) 71)+, intros add: more_intros, solve_triv+)
+  done
+
+lemma n_ps_rangeD:
+  "p < n_ps" if "p \<in> set ps" "set ps \<subseteq> {0..<n_ps}"
+  using that by auto
+
+lemma conv_trans_broad:
+  "conv.trans_broad = (\<lambda>(l, g, a, r, l'). (l, map conv_ac g, a, r, l')) ` trans_broad"
+  unfolding conv.trans_broad_alt_def trans_broad_alt_def
+  apply standard
+   supply [simp] = L_len
+  subgoal
+  proof -
+    have **: "\<exists> gs'. gs = conv_cc o gs' \<and>
+          (\<forall>p\<in>set ps.(L ! p, gs' p, In a, fs p, rs p, ls' p) \<in> trans (N p))"
+      if assms:
+        "\<forall>p\<in>set ps. (L ! p, gs p, In a, fs p, rs p, ls' p) \<in> trans (conv.N p)"
+        "set ps \<subseteq> {0..<n_ps}" "\<forall>p. p \<notin> set ps \<longrightarrow> gs p = []"
+      for L ps gs a fs rs ls'
+    proof -
+      have *: "gs p = conv_cc (Hilbert_Choice.inv conv_cc (gs p))" if "p \<in> set ps" for p
+        using that assms by (auto 4 3 simp: f_inv_into_f dest!: 73)
+      show ?thesis
+        apply (inst_existentials "Hilbert_Choice.inv conv_cc o gs")
+        subgoal
+          apply (rule ext)
+          subgoal for p
+            apply (cases "p \<in> set ps")
+            subgoal
+              by (simp, erule *)
+            subgoal
+              using that(3) by (auto intro: injI inv_f_eq conv_ac_inj)
+            done
+          done
+        subgoal
+          using that * by (force dest!: conv_cc_inj 73)
+        done
+    qed
+    have *: "set ps \<subseteq> {0..<n_ps} \<longleftrightarrow> (\<forall>p \<in> set ps. p < n_ps)" for ps
+      by auto
+    show ?thesis
+      apply (rule subsetI)
+      apply (clarsimp simp add: 3 9 10 broadcast_def split: prod.split_asm)
+      apply (drule (2) **)
+      apply (drule (1) 73)+
+      apply elims
+      apply (intro image_eqI[rotated] CollectI exI conjI)
+                        apply solve_triv+
+      subgoal premises prems \<comment>\<open>Commited\<close>
+        using prems(2) \<open>set _ \<subseteq> {0..<n_ps}\<close> by (auto dest: n_ps_rangeD simp: 9)
+      subgoal premises prems for L s s' s'' ae p g f r l' gs fs rs ls' ps gs' g' \<comment>\<open>Maximal set\<close>
+        using prems(3,17-) 71 by blast
+      by solve_triv+ (simp split: prod.split add: map_concat)
+  qed
+  subgoal
+    apply (rule subsetI)
+    apply (clarsimp simp:
+        Simple_Network_Language.conv_t_def 3 7 9[symmetric] 10 broadcast_def map_concat)
+    apply (drule (1) 71)
+    apply (intros add: more_intros)
+                   apply solve_triv+
+               apply (subst comp_def; rule 71; fast elim: n_ps_rangeD; fail)
+    subgoal premises prems for L s s' s'' aj p g f r l' gs fs rs ls' ps
+      using prems(3,6) 9 by fastforce
+    subgoal premises prems for L s s' s'' aj p g f r l' gs fs rs ls' ps q ga fa ra l'a
+      using prems(4,9-) 9 by auto
+    by (solve_triv | blast)+
+  done
+
+lemma conv_prod_ta:
+  "conv.prod_ta = Normalized_Zone_Semantics_Impl.conv_A prod_ta"
+  unfolding conv.prod_ta_def prod_ta_def
+  unfolding conv.trans_prod_def trans_prod_def
+  unfolding conv.prod_inv_def prod_inv_def
+  unfolding conv.N_def N_def 3
+  apply simp
+  apply (rule conjI)
+  subgoal
+    unfolding image_Un
+    by ((fo_rule arg_cong2)+; rule conv_trans_int conv_trans_bin conv_trans_broad)
+  subgoal \<comment>\<open>Invariant\<close>
+    unfolding conv.N_def N_def
+    by (rule ext) (auto simp: 5 map_concat intro!: map_cong arg_cong[where f = concat])
+  done
+
+end (* Anonymous context for private lemmas *)
+
+paragraph \<open>Fundamentals\<close>
 
 definition "clkp_set' \<equiv>
     (\<Union> A \<in> set automata. UNION (set (snd (snd A))) (collect_clock_pairs o snd))
@@ -71,10 +1061,6 @@ definition clk_set'  where
   \<open>clk_set'  =
   fst ` clkp_set' \<union>
   (\<Union> A \<in> set automata. \<Union> (_, _, _, _, r, _) \<in> set (fst (snd A)). set r)\<close>
-
-lemma N_eq:
-  \<open>N i = automaton_of (automata ! i)\<close> if \<open>i < n_ps\<close>
-  using that unfolding N_def n_ps_def fst_conv snd_conv by (intro nth_map; simp)
 
 lemma collect_clock_pairs_invsI:
   "(a, b) \<in> \<Union> ((collect_clock_pairs o snd) ` set invs)"
@@ -105,15 +1091,9 @@ lemma mem_trans_N_iff:
   "t \<in> Simple_Network_Language.trans (N i) \<longleftrightarrow> t \<in> set (fst (snd (automata ! i)))" if "i < n_ps"
   unfolding N_eq[OF that] by (auto split: prod.splits simp: automaton_of_def)
 
-paragraph \<open>Fundamentals\<close>
-
 lemma length_automata_eq_n_ps:
   "length automata = n_ps"
   unfolding n_ps_def by simp
-
-lemma L_len[intro, dest]:
-  "length L = n_ps" if "L \<in> states"
-  using that unfolding states_def by simp
 
 lemma clkp_set'_subs:
   "Timed_Automata.clkp_set prod_ta \<subseteq> clkp_set'"
@@ -212,26 +1192,31 @@ proof -
   ultimately show ?thesis by - (drule finite_subset; auto)
 qed
 
+definition (in Prod_TA_Defs)
+  "loc_set =
+  (\<Union> {fst ` trans (N p) | p. p < n_ps} \<union>
+        \<Union> {(snd o snd \<circ> snd \<circ> snd \<circ> snd) ` trans (N p) | p. p < n_ps})"
+
+lemma (in Prod_TA_Defs) states_loc_set:
+  "states \<subseteq> {L. set L \<subseteq> loc_set \<and> length L = n_ps}"
+  unfolding states_def loc_set_def
+  apply (intros add: more_intros)
+   apply (elims add: more_elims)
+   apply (drule mem_nth)
+   apply simp
+   apply (elims add: allE, assumption)
+   apply (simp split: prod.split_asm)
+   apply (erule disjE; (intros add: disjI1 disjI2 more_intros, solve_triv+); fail)
+  by (elims add: more_elims)
+
 lemma (in Prod_TA_Defs) finite_states:
   assumes finite_trans: "\<forall>p < n_ps. finite (Simple_Network_Language.trans (N p))"
   shows "finite states"
 proof -
-  have "states \<subseteq> {L.
-      set L \<subseteq>
-        (\<Union> {fst ` trans (N p) | p. p < n_ps} \<union>
-        \<Union> {(snd o snd \<circ> snd \<circ> snd \<circ> snd) ` trans (N p) | p. p < n_ps})
-        \<and> length L = n_ps}"
-    unfolding states_def
-    apply (intros add: more_intros)
-    apply (elims add: more_elims)
-     apply (drule mem_nth)
-     apply simp
-     apply (elims add: allE, assumption)
-     apply (simp split: prod.split_asm)
-     apply (erule disjE; (intros add: disjI1 disjI2 more_intros, solve_triv+); fail)
-    by (elims add: more_elims)
+  have "states \<subseteq> {L. set L \<subseteq> loc_set \<and> length L = n_ps}"
+    by (rule states_loc_set)
   also from finite_trans have "finite \<dots>"
-    by (intro finite_intros) auto
+    unfolding loc_set_def by (intro finite_intros) auto
   finally show ?thesis .
 qed
 
@@ -423,6 +1408,11 @@ fun vars_of_exp where
 | "vars_of_exp (var x) = {x}"
 | "vars_of_exp (if_then_else b e1 e2) = vars_of_bexp b \<union> vars_of_exp e1 \<union> vars_of_exp e2"
 
+definition (in Prod_TA_Defs)
+  "var_set =
+  (\<Union>S \<in> {(fst \<circ> snd \<circ> snd \<circ> snd) ` trans (N p) | p. p < n_ps}.
+    \<Union>f \<in> S. \<Union> (x, e) \<in> set f. {x} \<union> vars_of_exp e)"
+
 locale Simple_Network_Impl_nat =
   Simple_Network_Impl automata
   for automata ::
@@ -439,7 +1429,7 @@ locale Simple_Network_Impl_nat =
     "\<forall>i < n_ps. let (_, _, inv) = (automata ! i) in \<forall> (x, _) \<in> set inv. x < num_states i"
   assumes var_set:
     "\<forall>(_, trans, _) \<in> set automata. \<forall>(_, _, _, f, _, _) \<in> set trans.
-      \<forall>(x, upd) \<in> set f. x < n_vs \<and> (\<forall> i \<in> vars_of_exp upd. i < n_vs)"
+      \<forall>(x, upd) \<in> set f. x < n_vs \<and> (\<forall>i \<in> vars_of_exp upd. i < n_vs)"
   assumes bounds:
     "\<forall> i < n_vs. fst (bounds' ! i) = i"
   assumes action_set:
@@ -479,5 +1469,743 @@ next
 qed
 
 end (* Simple Network Impl nat *)
+
+
+
+
+
+
+
+
+(*
+locale TA_Renum =
+  fixes A :: "('a, 'c, int, 's) ta"
+    and renum_act   :: "'a \<Rightarrow> 'a1"
+    and renum_clock :: "'c \<Rightarrow> 'c1"
+    and renum_state :: "'s \<Rightarrow> 's1"
+  assumes renum_state_inj: "inj_on renum_state (Simulation_Graphs_TA.state_set A)"
+      and renum_clock_inj: "inj renum_clock"
+begin
+
+definition
+  "renum_cconstraint = map (map_acconstraint renum_clock id)"
+
+definition A' :: "('a1, 'c1, int, 's1) ta" where
+   "A' \<equiv> (
+    (\<lambda>(l, g, a, r, l').
+      (renum_state l, renum_cconstraint g, renum_act a, map renum_clock r, renum_state l'))
+    ` trans_of A,
+    renum_cconstraint o inv_of A o the_inv_into (Simulation_Graphs_TA.state_set A) renum_state
+  )"
+
+definition
+  "map_u u = u o the_inv renum_clock"
+
+lemma map_u_add:
+  "map_u (u \<oplus> d) = map_u u \<oplus> d"
+  by (auto simp: map_u_def cval_add_def)
+
+lemma renum_state_inv[simp]:
+  "the_inv_into (Simulation_Graphs_TA.state_set A) renum_state (renum_state l) = l"
+  if "l \<in> Simulation_Graphs_TA.state_set A"
+  using that by (intro the_inv_into_f_f renum_state_inj)
+
+lemma renum_state_eqD:
+  assumes "renum_state l = renum_state l'"
+    "l \<in> Simulation_Graphs_TA.state_set A" "l' \<in> Simulation_Graphs_TA.state_set A"
+  shows "l = l'"
+  using assms renum_state_inj by (meson inj_onD)
+
+definition clk_set where "clk_set \<equiv> Timed_Automata.clk_set A"
+
+lemma map_u_renum_clock[simp]:
+  "map_u u (renum_clock c) = u c" (* if "c \<in> clk_set" *)
+  using that unfolding map_u_def by (simp add: the_inv_into_f_f renum_clock_inj clk_set_def)
+
+lemma
+  assumes "u \<turnstile>\<^sub>a conv_ac ac" (* "constraint_clk ac \<in> clk_set" *)
+  shows "map_u u \<turnstile>\<^sub>a conv_ac (map_acconstraint renum_clock id ac)"
+  using assms by (cases ac) auto
+
+lemma
+  assumes "map_u u \<turnstile>\<^sub>a conv_ac (map_acconstraint renum_clock id ac)" "constraint_clk ac \<in> clk_set"
+  shows "u \<turnstile>\<^sub>a conv_ac ac"
+  using assms by (cases ac) auto
+
+lemma clock_val_a_renum_iff:
+  "map_u u \<turnstile>\<^sub>a conv_ac (map_acconstraint renum_clock id ac) = u \<turnstile>\<^sub>a conv_ac ac"
+  (* if "constraint_clk ac \<in> clk_set" *)
+  using that by (cases ac) auto
+
+lemma inv_1:
+  assumes
+    "\<forall>x\<in>set (inv_of A l). u \<turnstile>\<^sub>a conv_ac x" "ac \<in> set (renum_cconstraint (inv_of A l))"
+    (* "constraint_clk ac \<in> renum_clock ` clk_set" *)
+  shows "map_u u \<turnstile>\<^sub>a conv_ac ac"
+  using assms
+  unfolding renum_cconstraint_def
+  by (auto simp: clock_val_a_renum_iff)
+
+lemma inv_2:
+  assumes
+    "\<forall>x\<in>set (renum_cconstraint (inv_of A l)). map_u u \<turnstile>\<^sub>a conv_ac x" "ac \<in> set (inv_of A l)"
+    "constraint_clk ac \<in> clk_set"
+  shows "u \<turnstile>\<^sub>a conv_ac ac"
+  using assms unfolding renum_cconstraint_def by (auto simp: clock_val_a_renum_iff)
+
+lemma A_unfold:
+  "A = (trans_of A, inv_of A)"
+  by (simp add: trans_of_def inv_of_def)
+
+context
+begin
+
+private definition conv_A where "conv_A = Normalized_Zone_Semantics_Impl.conv_A"
+
+lemma inv_of_unfold:
+  "inv_of (conv_A B) = conv_cc o inv_of B" for B
+  unfolding conv_A_def inv_of_def by (simp split: prod.split)
+
+lemma trans_of_unfold:
+  "trans_of (conv_A B) = conv_t ` trans_of B" for B
+  unfolding conv_A_def trans_of_def by (simp split: prod.split)
+
+lemma inv_of_A':
+  "inv_of A' = renum_cconstraint o inv_of A o the_inv_into (Simulation_Graphs_TA.state_set A) renum_state"
+  unfolding A'_def inv_of_def by simp
+
+lemma map_u_cval_addD:
+  "u' = u \<oplus> d" if "map_u u' = map_u u \<oplus> d"
+  using that unfolding cval_add_def
+  apply (intro ext)
+  subgoal for c
+    apply (drule cong[OF _ HOL.refl, where x = "renum_clock c"])
+     apply auto
+    done
+  done
+
+lemma map_u_cval_addD:
+  "u' = u \<oplus> d" if "map_u u' = map_u u \<oplus> d" "\<forall>c. c \<notin> clk_set  \<longrightarrow> u' c = u c + d"
+  using that unfolding cval_add_def
+  apply (intro ext)
+  subgoal for c
+    apply (drule cong[OF _ HOL.refl, where x = "renum_clock c"])
+    apply (cases "c \<in> clk_set")
+    apply auto
+    done
+  oops
+
+lemma step_t_iff[unfolded conv_A_def]:
+  assumes
+    "l \<in> Simulation_Graphs_TA.state_set A" "l' \<in> Simulation_Graphs_TA.state_set A"
+  shows
+  "conv_A A' \<turnstile> \<langle>renum_state l, map_u u\<rangle> \<rightarrow>\<^bsup>d\<^esup> \<langle>renum_state l', map_u u'\<rangle> \<longleftrightarrow>
+   conv_A A \<turnstile> \<langle>l, u\<rangle> \<rightarrow>\<^bsup>d\<^esup> \<langle>l', u'\<rangle>"
+  using assms
+  apply -
+  apply standard
+  subgoal
+apply (cases rule: step_t.cases)
+     apply assumption
+    apply (auto simp: inv_of_unfold inv_of_A' split: prod.split_asm dest!: renum_state_eqD map_u_cval_addD)
+    apply rule
+     apply (auto simp: clock_val_def list_all_iff renum_state_inj inv_of_unfold inv_of_A' dest!: map_u_cval_addD renum_state_eqD)
+    apply (rule inv_2[rotated], assumption)
+    subgoal
+      sorry
+    apply (simp add: map_u_add)
+    done
+  subgoal
+    apply (cases rule: step_t.cases)
+     apply assumption
+    apply (auto simp: inv_of_unfold map_u_add split: prod.split_asm)
+    apply rule
+    apply (auto simp: clock_val_def list_all_iff renum_state_inj inv_of_unfold inv_of_A')
+    apply (drule (1) inv_1)
+    by (simp add: map_u_add)
+  done
+
+end (* Anonymous context for private definitions *)
+
+end (* TA Renum *)
+*)
+
+locale TA_Renum =
+  fixes A :: "('a, 'c, int, 's) ta"
+    and renum_act   :: "'a \<Rightarrow> 'a1"
+    and renum_clock :: "'c \<Rightarrow> 'c1"
+    and renum_state :: "'s \<Rightarrow> 's1"
+  assumes renum_state_inj: "inj renum_state"
+      and renum_clock_inj: "inj renum_clock"
+begin
+
+definition
+  "renum_cconstraint = map (map_acconstraint renum_clock id)"
+
+definition A' :: "('a1, 'c1, int, 's1) ta" where
+   "A' \<equiv> (
+    (\<lambda>(l, g, a, r, l').
+      (renum_state l, renum_cconstraint g, renum_act a, map renum_clock r, renum_state l'))
+    ` trans_of A,
+    renum_cconstraint o inv_of A o the_inv renum_state
+  )"
+
+definition
+  "map_u u = u o the_inv renum_clock"
+
+lemma map_u_add:
+  "map_u (u \<oplus> d) = map_u u \<oplus> d"
+  by (auto simp: map_u_def cval_add_def)
+
+lemma renum_state_inv[simp]:
+  "the_inv renum_state (renum_state l) = l"
+  by (intro the_inv_f_f renum_state_inj)
+
+lemma renum_state_eqD:
+  assumes "renum_state l = renum_state l'"
+  shows "l = l'"
+  using assms renum_state_inj by (meson inj_D)
+
+definition clk_set where "clk_set \<equiv> Timed_Automata.clk_set A"
+
+lemma map_u_renum_clock[simp]:
+  "map_u u (renum_clock c) = u c" (* if "c \<in> clk_set" *)
+  using that unfolding map_u_def by (simp add: the_inv_into_f_f renum_clock_inj clk_set_def)
+
+lemma
+  assumes "u \<turnstile>\<^sub>a conv_ac ac" (* "constraint_clk ac \<in> clk_set" *)
+  shows "map_u u \<turnstile>\<^sub>a conv_ac (map_acconstraint renum_clock id ac)"
+  using assms by (cases ac) auto
+
+lemma
+  assumes "map_u u \<turnstile>\<^sub>a conv_ac (map_acconstraint renum_clock id ac)" "constraint_clk ac \<in> clk_set"
+  shows "u \<turnstile>\<^sub>a conv_ac ac"
+  using assms by (cases ac) auto
+
+lemma clock_val_a_renum_iff:
+  "map_u u \<turnstile>\<^sub>a conv_ac (map_acconstraint renum_clock id ac) = u \<turnstile>\<^sub>a conv_ac ac"
+  (* if "constraint_clk ac \<in> clk_set" *)
+  using that by (cases ac) auto
+
+lemma inv_1:
+  assumes
+    "\<forall>x\<in>set (inv_of A l). u \<turnstile>\<^sub>a conv_ac x" "ac \<in> set (renum_cconstraint (inv_of A l))"
+    (* "constraint_clk ac \<in> renum_clock ` clk_set" *)
+  shows "map_u u \<turnstile>\<^sub>a conv_ac ac"
+  using assms
+  unfolding renum_cconstraint_def
+  by (auto simp: clock_val_a_renum_iff)
+
+lemma inv_2:
+  assumes
+    "\<forall>x\<in>set (renum_cconstraint (inv_of A l)). map_u u \<turnstile>\<^sub>a conv_ac x" "ac \<in> set (inv_of A l)"
+    "constraint_clk ac \<in> clk_set"
+  shows "u \<turnstile>\<^sub>a conv_ac ac"
+  using assms unfolding renum_cconstraint_def by (auto simp: clock_val_a_renum_iff)
+
+lemma A_unfold:
+  "A = (trans_of A, inv_of A)"
+  by (simp add: trans_of_def inv_of_def)
+
+context
+begin
+
+private definition conv_A where "conv_A = Normalized_Zone_Semantics_Impl.conv_A"
+
+lemma inv_of_unfold:
+  "inv_of (conv_A B) = conv_cc o inv_of B" for B
+  unfolding conv_A_def inv_of_def by (simp split: prod.split)
+
+lemma trans_of_unfold:
+  "trans_of (conv_A B) = conv_t ` trans_of B" for B
+  unfolding conv_A_def trans_of_def by (simp split: prod.split)
+
+lemma inv_of_A':
+  "inv_of A' = renum_cconstraint o inv_of A o the_inv renum_state"
+  unfolding A'_def inv_of_def by simp
+
+lemma map_u_cval_addD:
+  "u' = u \<oplus> d" if "map_u u' = map_u u \<oplus> d"
+  using that unfolding cval_add_def
+  apply (intro ext)
+  subgoal for c
+    apply (drule cong[OF _ HOL.refl, where x = "renum_clock c"])
+     apply auto
+    done
+  done
+
+lemma map_u_cval_addD:
+  "u' = u \<oplus> d" if "map_u u' = map_u u \<oplus> d" "\<forall>c. c \<notin> clk_set  \<longrightarrow> u' c = u c + d"
+  using that unfolding cval_add_def
+  apply (intro ext)
+  subgoal for c
+    apply (drule cong[OF _ HOL.refl, where x = "renum_clock c"])
+    apply (cases "c \<in> clk_set")
+    apply auto
+    done
+  oops
+
+lemma step_t_iff[unfolded conv_A_def]:
+  assumes
+    "l \<in> Simulation_Graphs_TA.state_set A" "l' \<in> Simulation_Graphs_TA.state_set A"
+  shows
+  "conv_A A' \<turnstile> \<langle>renum_state l, map_u u\<rangle> \<rightarrow>\<^bsup>d\<^esup> \<langle>renum_state l', map_u u'\<rangle> \<longleftrightarrow>
+   conv_A A \<turnstile> \<langle>l, u\<rangle> \<rightarrow>\<^bsup>d\<^esup> \<langle>l', u'\<rangle>"
+  using assms
+  apply -
+  apply standard
+  subgoal
+apply (cases rule: step_t.cases)
+     apply assumption
+    apply (auto simp: inv_of_unfold inv_of_A' split: prod.split_asm dest!: renum_state_eqD map_u_cval_addD)
+    apply rule
+     apply (auto simp: clock_val_def list_all_iff renum_state_inj inv_of_unfold inv_of_A' dest!: map_u_cval_addD renum_state_eqD)
+    apply (rule inv_2[rotated], assumption)
+    subgoal
+      sorry
+    apply (simp add: map_u_add)
+    done
+  subgoal
+    apply (cases rule: step_t.cases)
+     apply assumption
+    apply (auto simp: inv_of_unfold map_u_add split: prod.split_asm)
+    apply rule
+    apply (auto simp: clock_val_def list_all_iff renum_state_inj inv_of_unfold inv_of_A')
+    apply (drule (1) inv_1)
+    by (simp add: map_u_add)
+  done
+
+end (* Anonymous context for private definitions *)
+
+end (* TA Renum *)
+
+no_notation
+  comp2  (infixl "\<circ>\<circ>" 55) and
+  comp3  (infixl "\<circ>\<circ>\<circ>" 55)
+
+locale Simple_Network_Rename =
+  Simple_Network_Impl automata for automata ::
+    "('s list \<times> (('a :: countable) act, 's, 'c, int, 'x :: countable, int) transition list
+      \<times> (('s :: countable) \<times> ('c :: countable, int) cconstraint) list) list"
+begin
+
+context
+  fixes renum_acts   :: "'a \<Rightarrow> nat"
+    and renum_vars   :: "'x \<Rightarrow> nat"
+    and renum_clocks :: "'c \<Rightarrow> nat"
+    and renum_states :: "nat \<Rightarrow> 's \<Rightarrow> nat"
+  assumes renum_states_inj:
+    "\<forall>i<n_ps. \<forall>x\<in>loc_set. \<forall>y\<in>loc_set. renum_states i x = renum_states i y \<longrightarrow> x = y"
+  and renum_clocks_inj:
+    "inj_on renum_clocks clk_set'"
+  and "inj_on renum_vars var_set"
+begin
+
+definition
+  "map_cconstraint f g xs = map (map_acconstraint f g) xs"
+
+definition
+  "extend_inj (f :: ('xx :: countable) \<Rightarrow> nat) S \<equiv> let m = Max ({0} \<union> f ` S) + 1 in
+    (\<lambda> x. if x \<in> S then f x else m + (SOME f. inj f) x)"
+
+lemma extend_inj_inj:
+  "inj (extend_inj f S)" if "inj_on f S" "finite S" for f :: "'b :: countable \<Rightarrow> nat"
+proof -
+  obtain g :: "'b \<Rightarrow> nat" where "inj g"
+    by auto
+  have *: "f x \<le> Max (insert 0 (f ` S))" if "x \<in> S" for x
+    using that \<open>finite S\<close> by auto
+  from that show ?thesis
+    apply (intro injI)
+    unfolding extend_inj_def
+    apply (auto split: if_split_asm dest: inj_onD *)
+    subgoal for x y
+      by (metis from_nat_to_nat to_nat_def)
+    done
+qed
+
+definition
+  "renum_cconstraint = map_cconstraint (extend_inj renum_clocks clk_set') id"
+
+definition
+  "renum_act = map_act renum_acts"
+
+definition
+  "renum_exp = map_exp (extend_inj renum_vars var_set) id"
+
+definition
+  "renum_upd = map (\<lambda>(x, upd). (extend_inj renum_vars var_set x, renum_exp upd))"
+
+definition
+  "renum_reset = map (extend_inj renum_clocks clk_set')"
+
+definition renum_automaton where
+  "renum_automaton i \<equiv> \<lambda>(commited, trans, inv). let
+    commited' = map (renum_states i) commited;
+    trans' = map (\<lambda>(l, g, a, upd, r, l').
+      (renum_states i l, renum_cconstraint g, renum_act a, renum_upd upd, renum_reset r, 
+      renum_states i l')
+    ) trans;
+    inv' = map (\<lambda>(l, g). (renum_states i l, renum_cconstraint g)) inv
+  in (commited', trans', inv')
+"
+
+interpretation renum: Simple_Network_Impl
+  "map_index renum_automaton automata"
+  "map renum_acts broadcast"
+  "map (\<lambda>(a,b,c). (renum_vars a, b, c)) bounds'"
+  "formula" .
+
+definition
+  "vars_inv \<equiv> the_inv (extend_inj renum_vars var_set)"
+
+definition
+  "map_st \<equiv> \<lambda>(L, s). (map_index ((\<lambda> r. extend_inj r loc_set) o renum_states) L, s o vars_inv)"
+
+definition
+  "clocks_inv \<equiv> the_inv (extend_inj renum_clocks clk_set')"
+
+definition
+  "map_u u = u o clocks_inv"
+
+lemma map_u_add[simp]:
+  "map_u (u \<oplus> d) = map_u u \<oplus> d"
+  by (auto simp: map_u_def cval_add_def)
+
+definition renum_label where
+  "renum_label = map_label renum_acts"
+
+lemma
+  "inj (map_index renum_states)"
+  apply (rule injI)
+  oops
+
+lemma states_loc_setD:
+  "set L \<subseteq> loc_set" if "L \<in> states"
+  using states_loc_set that by auto
+
+lemma renum_states_inj_states:
+  assumes "map_index renum_states L = map_index renum_states L'" "L \<in> states" "L' \<in> states"
+  shows "L = L'"
+  using assms
+  apply -
+  apply (rule map_index_inj[where S = loc_set and T = loc_set])
+  subgoal
+    apply (simp add: L_len)
+    done
+     apply assumption
+  apply (erule states_loc_setD)
+   apply (erule states_loc_setD)
+  apply (simp add: L_len renum_states_inj)
+  done
+
+lemma renum_vars_inj:
+  assumes
+  "(s \<circ> vars_inv) = (s' \<circ> vars_inv)"
+shows
+  "s = s'"
+  apply (rule ext)
+  subgoal for x
+    using assms apply -
+    thm cong[OF _ HOL.refl, where x = x]
+    apply (drule cong[OF _ HOL.refl, where x = "renum_vars x"])
+    apply (simp add: vars_inv_def)
+    sorry
+  sorry
+
+interpretation ta_renum: TA_Renum
+  prod_ta
+  renum_label
+  "extend_inj renum_clocks clk_set'"
+  map_st
+  apply standard
+  subgoal
+    unfolding map_st_def
+    apply (rule inj_onI)
+    apply clarsimp
+    apply (rule conjI)
+    subgoal for L s L' s'
+      apply (erule renum_states_inj_states)
+      subgoal
+        sorry
+        sorry
+      subgoal for L s L' s'
+        by (rule renum_vars_inj)
+      done
+  sorry
+
+no_notation
+  comp2  (infixl "\<circ>\<circ>" 55) and
+  comp3  (infixl "\<circ>\<circ>\<circ>" 55)
+
+lemma inv_map_stD:
+  assumes "the_inv map_st (L, s) = (L', s')"
+  shows "map_index ((\<lambda> r. extend_inj r loc_set) o renum_states) L'  = L"
+  sorry
+
+lemma ta_renum_A'_eq:
+  "ta_renum.A' = renum.prod_ta"
+  unfolding ta_renum.A'_def renum.prod_ta_def
+  apply rule
+  apply rule
+  subgoal
+    unfolding renum.trans_prod_def
+    sorry
+  subgoal
+    unfolding prod_ta_def
+    print_antiquotations
+    thm prod_inv_def
+    unfolding renum.prod_inv_def prod_inv_def
+    apply (rule ext)
+    subgoal for x
+      apply (cases x)
+      subgoal for L s
+unfolding case_prod_conv inv_of_def
+  apply (simp only: )
+  unfolding case_prod_conv inv_of_def fst_conv snd_conv
+  unfolding comp_def
+  apply (cases "the_inv map_st (L, s)")
+  apply (simp only: case_prod_conv)
+  unfolding ta_renum.renum_cconstraint_def
+  unfolding map_concat map_map
+  apply (fo_rule arg_cong)
+  apply (rule map_cong)
+  subgoal
+    sorry
+  unfolding comp_def
+  unfolding renum.N_def N_def fst_conv snd_conv
+  apply (drule inv_map_stD)
+  unfolding map_st_def
+  unfolding case_prod_conv
+  apply (simp only: case_prod_conv)
+apply (simp only: )
+
+
+  oops
+  sorry
+
+lemma ta_renum_map_u_eq:
+  "ta_renum.map_u = map_u"
+  unfolding ta_renum.map_u_def map_u_def clocks_inv_def ..
+
+lemma
+  "Normalized_Zone_Semantics_Impl.conv_A prod_ta \<turnstile> \<langle>l, u\<rangle> \<rightarrow>\<^bsup>d\<^esup> \<langle>l', u'\<rangle>
+\<longleftrightarrow> Normalized_Zone_Semantics_Impl.conv_A renum.prod_ta \<turnstile> \<langle>map_st l, map_u u\<rangle> \<rightarrow>\<^bsup>d\<^esup> \<langle>map_st l', map_u u'\<rangle>"
+  apply (subst ta_renum.step_t_iff[symmetric])
+
+  apply (subst ta_renum_A'_eq)
+  apply (simp add: ta_renum_A'_eq ta_renum_map_u_eq)
+  done
+  thm ta_renum.step_t_iff
+  oops
+proof -
+  define A  where "A  \<equiv> Normalized_Zone_Semantics_Impl.conv_A prod_ta"
+  define A' where "A' \<equiv> Normalized_Zone_Semantics_Impl.conv_A renum.prod_ta"
+  show ?thesis
+    unfolding A_def[symmetric] A'_def[symmetric]
+  apply standard
+   apply (erule step_t.cases)
+  apply simp
+  apply (rule step_t.intros)
+
+term prod_ta
+
+lemma
+  "Bisimulation_Invariant
+
+"
+
+
+
+interpretation nat: Simple_Network_Impl_nat
+  "map renum_acts broadcast"
+  "map (\<lambda>(a,b,c). (renum_vars a, b, c)) bounds'"
+  "formula"
+  "map_index renum_automaton automata"
+  m
+  num_states
+  num_actions
+  apply standard
+
+
+end
+
+
+context Simple_Network_Impl
+begin
+
+context
+  fixes renum_acts   :: "'a \<Rightarrow> nat"
+    and renum_vars   :: "'x \<Rightarrow> nat"
+    and renum_clocks :: "'c \<Rightarrow> nat"
+    and renum_states :: "nat \<Rightarrow> 's \<Rightarrow> nat"
+  assumes renum_states_inj:
+    "\<forall>i<n_ps. \<forall>x\<in>loc_set. \<forall>y\<in>loc_set. renum_states i x = renum_states i y \<longrightarrow> x = y"
+and "\<forall>v \<in>"
+begin
+
+definition
+  "map_cconstraint f g xs = map (map_acconstraint f g) xs"
+
+definition
+  "renum_cconstraint = map_cconstraint renum_clocks id"
+
+definition
+  "renum_act = map_act renum_acts"
+
+definition
+  "renum_exp = map_exp renum_vars id"
+
+definition
+  "renum_upd = map (\<lambda>(x, upd). (renum_vars x, renum_exp upd))"
+
+definition
+  "renum_reset = map renum_clocks"
+
+definition renum_automaton where
+  "renum_automaton i \<equiv> \<lambda>(commited, trans, inv). let
+    commited' = map (renum_states i) commited;
+    trans' = map (\<lambda>(l, g, a, upd, r, l').
+      (renum_states i l, renum_cconstraint g, renum_act a, renum_upd upd, renum_reset r, 
+      renum_states i l')
+    ) trans;
+    inv' = map (\<lambda>(l, g). (renum_states i l, renum_cconstraint g)) inv
+  in (commited', trans', inv')
+"
+
+interpretation renum: Simple_Network_Impl
+  "map_index renum_automaton automata"
+  "map renum_acts broadcast"
+  "map (\<lambda>(a,b,c). (renum_vars a, b, c)) bounds'"
+  "formula" .
+
+definition
+  "vars_inv \<equiv> the_inv renum_vars"
+
+definition
+  "map_st \<equiv> \<lambda>(L, s). (map_index renum_states L, s o vars_inv)"
+
+definition
+  "clocks_inv \<equiv> the_inv renum_clocks"
+
+definition
+  "map_u u = u o clocks_inv"
+
+lemma map_u_add[simp]:
+  "map_u (u \<oplus> d) = map_u u \<oplus> d"
+  by (auto simp: map_u_def cval_add_def)
+
+definition renum_label where
+  "renum_label = map_label renum_acts"
+
+lemma
+  "inj (map_index renum_states)"
+  apply (rule injI)
+  oops
+
+lemma states_loc_setD:
+  "set L \<subseteq> loc_set" if "L \<in> states"
+  using states_loc_set that by auto
+
+lemma renum_states_inj_states:
+  assumes "map_index renum_states L = map_index renum_states L'" "L \<in> states" "L' \<in> states"
+  shows "L = L'"
+  using assms
+  apply -
+  apply (rule map_index_inj[where S = loc_set and T = loc_set])
+  subgoal
+    apply (simp add: L_len)
+    done
+     apply assumption
+  apply (erule states_loc_setD)
+   apply (erule states_loc_setD)
+  apply (simp add: L_len renum_states_inj)
+  done
+
+lemma renum_vars_inj:
+  assumes
+  "(s \<circ>\<circ> Simple_Network_Impl.vars_inv) renum_vars = (s' \<circ>\<circ> Simple_Network_Impl.vars_inv) renum_vars"
+shows
+  "s = s'"
+  apply (rule ext)
+  subgoal for x
+    using assms apply -
+    thm cong[OF _ HOL.refl, where x = x]
+    apply (drule cong[OF _ HOL.refl, where x = "renum_vars x"])
+    apply (simp add: vars_inv_def)
+    sorry
+  sorry
+
+interpretation ta_renum: TA_Renum
+  prod_ta
+renum_label
+renum_clocks
+map_st
+  apply standard
+  subgoal
+    unfolding map_st_def
+    apply (rule inj_onI)
+    apply clarsimp
+    apply (rule conjI)
+    subgoal for L s L' s'
+      apply (erule renum_states_inj_states)
+      subgoal
+        sorry
+        sorry
+      subgoal for L s L' s'
+
+    sorry
+  sorry
+
+lemma ta_renum_A'_eq:
+  "ta_renum.A' = renum.prod_ta"
+  sorry
+
+lemma ta_renum_map_u_eq:
+  "ta_renum.map_u = map_u"
+  unfolding ta_renum.map_u_def map_u_def clocks_inv_def ..
+
+lemma
+  "Normalized_Zone_Semantics_Impl.conv_A prod_ta \<turnstile> \<langle>l, u\<rangle> \<rightarrow>\<^bsup>d\<^esup> \<langle>l', u'\<rangle>
+\<longleftrightarrow> Normalized_Zone_Semantics_Impl.conv_A renum.prod_ta \<turnstile> \<langle>map_st l, map_u u\<rangle> \<rightarrow>\<^bsup>d\<^esup> \<langle>map_st l', map_u u'\<rangle>"
+  apply (subst ta_renum.step_t_iff[symmetric])
+  apply (subst ta_renum_A'_eq)
+  apply (simp add: ta_renum_A'_eq ta_renum_map_u_eq)
+  done
+  thm ta_renum.step_t_iff
+  oops
+proof -
+  define A  where "A  \<equiv> Normalized_Zone_Semantics_Impl.conv_A prod_ta"
+  define A' where "A' \<equiv> Normalized_Zone_Semantics_Impl.conv_A renum.prod_ta"
+  show ?thesis
+    unfolding A_def[symmetric] A'_def[symmetric]
+  apply standard
+   apply (erule step_t.cases)
+  apply simp
+  apply (rule step_t.intros)
+
+term prod_ta
+
+lemma
+  "Bisimulation_Invariant
+
+"
+
+
+
+interpretation nat: Simple_Network_Impl_nat
+  "map renum_acts broadcast"
+  "map (\<lambda>(a,b,c). (renum_vars a, b, c)) bounds'"
+  "formula"
+  "map_index renum_automaton automata"
+  m
+  num_states
+  num_actions
+  apply standard
+
+
+end
+
+end
 
 end (* Theory *)
